Otway-Rees: more progress - verified all protocol steps
Now the valid_session preds of the final initiator and responder state can be
used to proof the secrecy of the key in the states of all honest principals.

otway-rees-fixed/OYRS.Protocol.fst
@@ -366,7 +366,6 @@ let responder_send_msg_4 b msg3_idx b_si =
                 let prev = now in
                 let event = event_forward_key c a b srv k_ab in
                 trigger_event #oyrs_preds b event;
-                admit();
 
                 // create and send fourth message
                 let msg4:message now = Msg4 c (|tag_ev_a,c_ev_a|) in
@@ -390,6 +389,14 @@ let responder_send_msg_4 b msg3_idx b_si =
                 includes_can_flow_lemma now [P b; P srv] [P b];
                 can_flow_transitive now (get_label oyrs_key_usages k_ab) (readers [P b; P srv]) (readers [P b]);
                 assert(is_msg oyrs_global_usage now k_ab (readers [P b]));
+                // prove responder or server corrupt or k_ab is labeled with server, initiator, responder
+                assert((exists c n_a. did_event_occur_before prev srv (event_send_key c a b srv n_a n_b k_ab))
+                  ==> (exists c n_a. did_event_occur_before now srv (event_send_key c a b srv n_a n_b k_ab)));
+                assert((corrupt_id now (P b)) \/ (corrupt_id now (P srv))
+                  \/ (exists c n_a. did_event_occur_before now srv (event_send_key c a b srv n_a n_b k_ab)));
+                assert((exists c n_a. did_event_occur_before now srv (event_send_key c a b srv n_a n_b k_ab))
+                  ==> was_rand_generated_before now k_ab (readers [P srv; P a; P b]) (aead_usage "sk_i_r"));
+                rand_is_secret #oyrs_global_usage #now #(readers [P srv; P a; P b]) #(aead_usage "sk_i_r") k_ab;
                 let ser_st = serialize_session_st now b b_si b_vi st_r_sent_m4 in
                 update_session #oyrs_preds #now b b_si b_vi ser_st;
 
@@ -422,16 +429,80 @@ let initiator_recv_msg_4 a msg4_idx a_si =
         else
           // decrypt part of message intended for initiator
           let now = global_timestamp () in
-          match aead_dec #oyrs_global_usage #now #(get_label oyrs_key_usages k_as) k_as (string_to_bytes #oyrs_global_usage #now "iv") c_ev_a (string_to_bytes #oyrs_global_usage #now "ev_i") with
+          let ad = (string_to_bytes #oyrs_global_usage #now "ev3_i") in
+          match aead_dec #oyrs_global_usage #now #(get_label oyrs_key_usages k_as) k_as (string_to_bytes #oyrs_global_usage #now "iv") c_ev_a ad with
           | Success ser_ev_a -> (
             // parse the decrypted part
             let tagged_ser_ev_a:ser_encval now (get_label oyrs_key_usages k_as) = (|tag_ev_a,ser_ev_a|) in
             match parse_encval tagged_ser_ev_a with
-            | Success (EncMsg3_I n_a' k_ab) -> (
+            | Success (EncMsg3_I n_a' b' k_ab) -> (
               parsed_encval_is_valid_lemma tagged_ser_ev_a;
 
               if n_a <> n_a' then error "i_recv_m4: initiator nonce in message does not match with the stored nonce\n"
+              else if b <> b' then error "i_recv_m4: stored responder does not match with responder in part encrypted for initiator\n"
               else
+                // k_as publishable or aead_pred holds
+                assert(is_publishable oyrs_global_usage now k_as
+                  \/ aead_pred oyrs_usage_preds now "sk_i_srv" k_as ser_ev_a ad);
+                // if k_as publishable, k_as readers flow to public
+                assert(is_publishable oyrs_global_usage now k_as
+                  ==> can_flow now (get_label oyrs_key_usages k_as) public);
+                // k_as readable by responder and server
+                assert(is_labeled oyrs_global_usage now k_as (readers [P a; P srv]));
+                // k_as readers flow to public -> k_as readers corrupted
+                publishable_readers_implies_corruption #now [P a; P srv];
+                // k_as readers corrupted or aead_pred holds
+                includes_corrupt_2_lemma now (P a) (P srv);
+                assert((corrupt_id now (P a)) \/ (corrupt_id now (P srv))
+                  \/ aead_pred oyrs_usage_preds now "sk_i_srv" k_as ser_ev_a ad);
+
+                // if aead_pred holds, oyrs_aead_pred holds for some timestamp before now
+                assert(aead_pred oyrs_usage_preds now "sk_i_srv" k_as ser_ev_a ad
+                  ==> (exists i. later_than now i /\ oyrs_aead_pred i "sk_i_srv" k_as ser_ev_a ad));
+                // k_as readers corrupted or oyrs_aead_pred holds for some timestamp before now
+                assert((corrupt_id now (P a)) \/ (corrupt_id now (P srv))
+                  \/ (exists i. later_than now i /\ oyrs_aead_pred i "sk_i_srv" k_as ser_ev_a ad));
+
+                // plug in definition of oyrs_aead_pred
+                assert(exists i. (later_than now i /\ oyrs_aead_pred i "sk_i_srv" k_as ser_ev_a ad)
+                  ==> (forall (t:string{CryptoLib.bytes_to_string ad = Success t}). can_aead_encrypt i "sk_i_srv" k_as (|t,ser_ev_a|) ad));
+                assert((corrupt_id now (P a)) \/ (corrupt_id now (P srv))
+                  \/ (exists i. forall (t:string{CryptoLib.bytes_to_string ad = Success t}). later_than now i /\ can_aead_encrypt i "sk_i_srv" k_as (|t,ser_ev_a|) ad));
+
+                // tag_ev_a is concrete value for t
+                assert(CryptoLib.bytes_to_string ad = Success tag_ev_a);
+                // can_aead_encrypt holds for all t -> holds for concrete t
+                can_aead_encrypt_encval_lemma now tag_ev_a (get_label oyrs_key_usages k_as) "sk_i_srv" k_as ser_ev_a ad;
+                // if can_aead_encrypt holds for all t, it holds for tag_ev_a
+                assert((exists i. forall (t:string{CryptoLib.bytes_to_string ad = Success t}). later_than now i /\ can_aead_encrypt i "sk_i_srv" k_as (|t,ser_ev_a|) ad)
+                  ==> (exists i. later_than now i /\ can_aead_encrypt i "sk_i_srv" k_as (|tag_ev_a,ser_ev_a|) ad));
+                // k_as readers corrupted or can_aead_encrypt holds for tag_ev_a
+                assert((corrupt_id now (P a)) \/ (corrupt_id now (P srv))
+                  \/ (exists i. later_than now i /\ can_aead_encrypt i "sk_i_srv" k_as (|tag_ev_a,ser_ev_a|) ad));
+
+                // prepare F* for rest of proof
+                (*** NOTE: THIS LEMMA IS NOT PART OF THE PUBLIC DY* VERSION ***)
+                readers_is_injective_2 a srv;
+                parse_encval_lemma #now #(get_label oyrs_key_usages k_as) (|tag_ev_a,ser_ev_a|);
+                assert(get_label oyrs_key_usages k_as == (readers [P a; P srv])
+                  /\ _parse_encval (|tag_ev_a,ser_ev_a|) == Success (EncMsg3_I n_a b k_ab));
+                assert((corrupt_id now (P a)) \/ (corrupt_id now (P srv))
+                  \/ (exists i. later_than now i /\ get_label oyrs_key_usages k_as == (readers [P a; P srv]) /\ (exists c n_b. did_event_occur_before i srv (event_send_key c a b srv n_a n_b k_ab))));
+
+                // if can_aead_encrypt holds for tag_ev_a, event_send_key occured before some timestamp before now
+                assert((exists i. later_than now i /\ can_aead_encrypt i "sk_i_srv" k_as (|tag_ev_a,ser_ev_a|) ad)
+                  ==> (exists i. later_than now i /\ (exists c n_b. did_event_occur_before i srv (event_send_key c a b srv n_a n_b k_ab))));
+                // k_as readers corrupted or event_send_key occured before some timestamp before now
+                assert((corrupt_id now (P a)) \/ (corrupt_id now (P srv))
+                  \/ (exists i. later_than now i /\ (exists c n_b. did_event_occur_before i srv (event_send_key c a b srv n_a n_b k_ab))));
+
+                // if event_send_key occured before some timestamp before now, it occured before now (AHOI, captain obvious)
+                assert((exists i c n_b. later_than now i /\ did_event_occur_before i srv (event_send_key c a b srv n_a n_b k_ab))
+                  ==> (exists c n_b. did_event_occur_before now srv (event_send_key c a b srv n_a n_b k_ab)));
+                // k_as readers corrupted or event_send_key occured before now
+                assert((corrupt_id now (P a)) \/ (corrupt_id now (P srv))
+                  \/ (exists c n_b. did_event_occur_before now srv (event_send_key c a b srv n_a n_b k_ab)));
+
                 // trigger event 'recv key'
                 let prev = now in
                 let event = event_recv_key c a b srv k_ab in
@@ -453,6 +524,14 @@ let initiator_recv_msg_4 a msg4_idx a_si =
                 includes_can_flow_lemma now [P a; P srv] [P a];
                 can_flow_transitive now (get_label oyrs_key_usages k_ab) (readers [P a; P srv]) (readers [P a]);
                 assert(is_msg oyrs_global_usage now k_ab (readers [P a]));
+                // prove responder or server corrupt or k_ab is labeled with server, initiator, responder
+                assert((exists c n_b. did_event_occur_before prev srv (event_send_key c a b srv n_a n_b k_ab))
+                  ==> (exists c n_b. did_event_occur_before now srv (event_send_key c a b srv n_a n_b k_ab)));
+                assert((corrupt_id now (P a)) \/ (corrupt_id now (P srv))
+                  \/ (exists c n_b. did_event_occur_before now srv (event_send_key c a b srv n_a n_b k_ab)));
+                assert((exists c n_b. did_event_occur_before now srv (event_send_key c a b srv n_a n_b k_ab))
+                  ==> was_rand_generated_before now k_ab (readers [P srv; P a; P b]) (aead_usage "sk_i_r"));
+                rand_is_secret #oyrs_global_usage #now #(readers [P srv; P a; P b]) #(aead_usage "sk_i_r") k_ab;
                 let ser_st = serialize_session_st now a a_si a_vi st_i_rcvd_m4 in
                 update_session #oyrs_preds #now a a_si a_vi ser_st;
 
